src/Find.thy
@@ -1,0 +1,68 @@
+theory Find 
+imports Frame Tree_stack (* FIXME for sktoi; move to kv *)
+begin
+
+type_synonym find_error = store_error
+
+type_synonym stk = "(page_ref * nat) list"
+
+datatype find_state_t = 
+  F_down "key * page_ref * stk" (* fs *)
+  | F_finished "page_ref * kvs_t * stk"
+
+type_synonym 'a M = "store \<Rightarrow> (store * ('a,find_error) rresult)"
+(* s \<Rightarrow> (s * ['a + e] ) *) 
+
+definition bind :: "('a \<Rightarrow> 'b M) \<Rightarrow> 'a M \<Rightarrow> 'b M" where
+"bind f v = (% s. (case v s of (s1,Error x) \<Rightarrow> (s1,Error x) | (s1,Ok y) \<Rightarrow> (f y s1)))"
+
+definition return :: "'a \<Rightarrow> 'a M" where
+"return x = (% s. (s,Ok x))"
+
+definition get_store :: "unit \<Rightarrow> store M" where
+"get_store _ = (% s. (s,Ok(s)))"
+
+(* FIXME the following should really only require one read from store, not two *)
+definition page_ref_to_frame :: "page_ref \<Rightarrow> frame M" where
+"page_ref_to_frame r = (
+  get_store () |>bind 
+  (% s. let f = Frame.page_ref_to_frame s r in 
+  case f of Error x \<Rightarrow> (% s1. (s1,Error x)) | Ok y \<Rightarrow> (% s1. (s1,Ok y)))
+)"
+
+definition step :: "find_state_t \<Rightarrow> find_state_t option M" where
+"step fs = (
+  case fs of 
+  F_finished _ \<Rightarrow> (return None)
+  | F_down(k,r,stk) \<Rightarrow> (
+    page_ref_to_frame r |>bind
+    (% f. case f of 
+      Node_frame (ks,rs) \<Rightarrow> (
+        let i = search_key_to_index ks k in
+        let r' = rs!i in
+        return(Some(F_down(k,r',(r,i)#stk)))
+      )
+      | Leaf_frame kvs \<Rightarrow> (return(Some(F_finished(r,kvs,stk))))
+)))"
+
+(* general recursive find *)
+type_synonym 'a trace = "nat \<Rightarrow> 'a"
+function find :: "find_state_t \<Rightarrow> (find_state_t option M) trace" where
+"find fs n = (
+  case n of 0 \<Rightarrow> (step fs)
+  | Suc n \<Rightarrow> (
+    (find fs n) |>bind
+    (% fs. case fs of
+    None \<Rightarrow> return None
+    | Some fs \<Rightarrow> (step fs)    
+)))
+"    
+by auto
+
+(* and prove for code extraction... but we really want the first place (if any) that we get F_finished FIXME express in terms of leaf, and rewrite using "current" state to next state *)
+
+definition find_def_2 :: bool where
+"find_def_2 = (! fs n. find fs n = (if n=0 then return (Some fs) else 
+  step fs|>bind (% fs'. case fs' of None \<Rightarrow> return None | Some fs' \<Rightarrow> find fs' (n-1))))"
+
+end
