src/Frame.thy
@@ -1,0 +1,18 @@
+theory Frame
+imports Key_value_types Store
+begin
+
+type_synonym frame_nf_t = "key list * page_ref list"
+
+datatype frame = Node_frame frame_nf_t | Leaf_frame kvs_t
+
+definition page_to_frame :: "page \<Rightarrow> frame" where "page_to_frame = failwith ''FIXME''"
+
+definition frame_to_page :: "frame \<Rightarrow> page" where "frame_to_page = failwith ''FIXME''"
+
+definition page_ref_to_frame :: "store \<Rightarrow> page_ref \<Rightarrow> frame M" where
+"page_ref_to_frame s r = (
+  page_ref_to_page s r |> rbind (% p. Ok (p|>page_to_frame))
+)"
+
+end
