src/Store.thy
@@ -1,0 +1,21 @@
+theory Store
+imports Util
+begin
+
+(* really these types are abstract *)
+datatype page_ref = Page_ref nat (* r *)
+datatype page = Page nat (* p *)
+datatype store = Store nat (* s *)
+
+datatype store_error = string (* e *)
+
+type_synonym 'a M = "('a,store_error) rresult" 
+
+definition "page_ref_to_page" :: "store \<Rightarrow> page_ref \<Rightarrow> page M" where
+"page_ref_to_page s p = failwith ''FIXME''"
+
+definition "allocate" :: "store \<Rightarrow> page \<Rightarrow> (store * page_ref)  M" where
+"allocate s p = failwith ''FIXME''"
+
+
+end
